(i) $\dq \Leftarrow \dq$ Sei $n \in \mathbb{N}_{0}$ und $x_{0},...,x_{n+1} \in E$ mit $\mathbb{P}[X_{0} = x_{0},...,X_{n} = x_{n}]>0$. Dann gilt
\begin{itemize}
\item $\mathbb{P}[X_{n+1} = x_{n+1} \: | \: X_{0} = x_{0},...,X_{n} = x_{n}]$
\begin{equation*}
=\dfrac{\mathbb{P}[X_{0} = x_{0},...,X_{n+1} = x_{n+1}]}{\mathbb{P}[X_{0} = x_{0},...,X_{n} = x_{n}]} = \dfrac{\nu(x_{0}) p(x_{0},x_{1}) \cdot ...\cdot p(x_{n-1},x_{n})p(x_{n},x_{n+1})}{\nu(x_{0}) p(x_{0},x_{1}) \cdot ...\cdot p(x_{n-1},x_{n})} = p(x_{n},x_{n+1})
\end{equation*}
\item $\mathbb{P}[X_{0} = x_{0}] = \nu(x_{0})$
\end{itemize}
Folglich ist ${(X_{n})}_{n \in \mathbb{N}_{0}}$ eine $(\nu,P)$-Markovkette.
\\
\\
$\dq \Rightarrow n\dq$ Beweis durch vollständige Induktion über  n
\\
\\
\textbf{IA}
\\
n=0 : $\mathbb{P}[X_{0} = x_{0}] \stackrel{\mathrm{Def.} \ref{zeithomogene Markovkette} \:        \mathrm{(ii)}}{=} \nu(x_{0})$
\\
n=1 : $\mathbb{P}[X_{0} = x_{0},X_{1} = x_{1}] = \mathbb{P}[X_{0} = x_{0}]\mathbb{P}[X_{1} = x_{1} \: | \: X_{0} = x_{0}]  \stackrel{\mathrm{Def.} \ref{zeithomogene Markovkette} \: \mathrm{(i),(ii)}}{=} \nu(x_{0})p(x_{0},x_{1})$
\\
\\
\textbf{IS} n $\to$ n+1
\\
Sei $\mathbb{P}[X_{0} = x_{0},...,X_{n} = x_{n}]>0$ (andernfalls sind beide Seiten identisch gleich 0).
\begin{equation*}
\mathbb{P}[X_{0} = x_{0},...,X_{n} = x_{n}, X_{n+1} = x_{n+1}]
\end{equation*}
\begin{equation*}
= \mathbb{P}[X_{0} = x_{0},...,X_{n} = x_{n}]\mathbb{P}[X_{n+1} = x_{n+1          }\: | \: X_{0} = x_{0},...,X_{n} = x_{n}]
\end{equation*}
\begin{equation*}
\stackrel{\mathrm{IV}}{=} \nu(x_{0}) p(x_{0},x_{1}) \cdot ...\cdot p(x_{n-1},x_{n})\mathbb{P}[X_{n+1} = x_{n+1}\: | \: X_{0} = x_{0},...,X_{n} = x_{n}]
\end{equation*}
\begin{equation*}
\stackrel{\mathrm{Def.}\ref{zeithomogene Markovkette} \: \mathrm{(i)}}{=} \nu(x_{0}) p(x_{0},x_{1}) \cdot ...\cdot p(x_{n-1},x_{n})p(x_{n},x_{n+1})
\end{equation*}
(ii) Für $n \in \mathbb{N}_{0}$ und $x,y \in E$ mit $\mathbb{P}[X_{n} = x]>0$
\begin{equation*}
\mathbb{P}[X_{n+1} = y \: | \: X_{n} = x] = \dfrac{\mathbb{P}[X_{0} \in E,.., X_{n-1} \in E, X_{n} = x, X_{n+1} = y]}{\mathbb{P}[X_{0} \in E,.., X_{n-1} \in E, X_{n} = x]}
\end{equation*}
\begin{equation*}
= \dfrac{\sum_{x_{0},..,x_{n-1}} \nu(x_{0}) p(x_{0},x_{1}) \cdot ...\cdot p(x_{n-1},x)p(x,y)}{\sum_{x_{0},..,x_{n-1}} \nu(x_{0}) p(x_{0},x_{1}) \cdot ...\cdot p(x_{n-1},x)} = p(x,y)
\end{equation*}